src/program_proof/simplepb/pb_init_proof.v
@@ -1,0 +1,52 @@
+From Perennial.base_logic Require Import lib.saved_prop.
+From Perennial.program_proof Require Import grove_prelude.
+From Goose.github_com.mit_pdos.gokv.simplepb Require Export pb.
+From Perennial.program_proof.simplepb Require Export pb_ghost.
+From Perennial.program_proof.simplepb Require Import pb_definitions.
+From Perennial.program_proof.grove_shared Require Import urpc_spec.
+
+Section pb_init_proof.
+
+Context {pb_record:PBRecord}.
+Notation OpType := (pb_OpType pb_record).
+Notation has_op_encoding := (pb_has_op_encoding pb_record).
+Notation has_snap_encoding := (pb_has_snap_encoding pb_record).
+Notation compute_reply := (pb_compute_reply pb_record).
+Notation pbG := (pbG (pb_record:=pb_record)).
+Context `{!gooseGlobalGS Σ}.
+Context `{!pbG Σ}.
+
+Lemma pb_server_init γsys :
+  is_proposal_lb γsys (U64 0) [] -∗
+  is_proposal_facts γsys (U64 0) [] ={⊤}=∗
+  ∃ γsrv,
+  own_Server_ghost γsys γsrv (U64 0) [] false.
+Proof.
+  (* Use pb_ghost_server_init from pb_ghost.v *)
+Admitted.
+
+Definition pb_spec_list γsys γsrv :=
+  [ (U64 0, ApplyAsBackup_spec γsys γsrv) ;
+    (U64 1, SetState_spec γsys γsrv) ;
+    (U64 2, GetState_spec γsys γsrv) ;
+    (U64 3, BecomePrimary_spec γsys γsrv);
+    (U64 4, Apply_spec γsys) ].
+
+Lemma pb_host_init host γsys γsrv :
+  host c↦ ∅ ={⊤}=∗
+  is_pb_host host γsys γsrv.
+Proof.
+  iIntros "Hchan".
+  iMod (handler_is_init_list2 host (pb_spec_list γsys γsrv) with "Hchan") as (γrpc) "H".
+  { simpl. set_solver. }
+  iModIntro.
+  rewrite is_pb_host_unfold.
+  iExists γrpc.
+  simpl.
+  iDestruct "H" as "(H1 & $ & $ & $ & $ & $ & _)".
+  iExactEq "H1".
+  f_equal.
+  set_solver.
+Qed.
+
+End pb_init_proof.
