src/program_proof/simplepb/pb_setstate_proof.v
@@ -50,9 +50,10 @@ Proof.
   wp_loadField.
   iDestruct (is_slice_to_small with "Henc_args_sl") as "Henc_args_sl".
   wp_apply (wp_frame_wand with "HΦ").
+  rewrite is_pb_host_unfold.
+  iNamed "Hsrv".
   wp_apply (wp_ReconnectingClient__Call2 with "Hcl_rpc [] Henc_args_sl Hrep").
   {
-    rewrite is_pb_host_unfold.
     iDestruct "Hsrv" as "[_ [$ _]]".
   }
   { (* Successful RPC *)
